a whole bunch of spaghetti for weakening of transfer

src-lite/wl_transfer.v
@@ -1,6 +1,9 @@
 Require Import worklist.
 Require Import decl_worklist.
 Require simplified_ind.
+Require Import lc.
+Require Import Program.Equality.
+Require Import list_properties.
 
 (*
 Inductive kind_iso : bkind → akind → Prop :=
@@ -110,6 +113,8 @@ Inductive lc_sse : ss_entry → Prop :=
 | lc_sse_kv : forall k, lc_sse (sse_kv k)
 .
 
+Hint Constructors lc_sse : core.
+
 Definition subst_set := list (var * ss_entry).
 
 Notation ": A !" :=
@@ -156,15 +161,29 @@ Inductive wf_ss : subst_set → Prop :=
   , wf_ss Θ → x `notin` dom Θ
   → wf_ss (Θ; x ≔ ⧼k⧽)
 | wf_ss_ex : forall x A e Θ
-  , wf_ss Θ
-  → x `notin` dom Θ → mono_btype e
+  , wf_ss Θ → x `notin` dom Θ
+  → lc_bexpr A → mono_btype e
   → wf_ss (Θ; x : A ≔ e)
 .
+
+Lemma wf_uniq : forall Θ,
+    wf_ss Θ → uniq Θ.
+Proof.
+  induction 1; eauto.
+Qed.
+
+#[export]
+Hint Resolve wf_uniq : core.
 
 Lemma wf_lc_sse : forall Θ x e,
   binds x e Θ → wf_ss Θ → lc_sse e.
 Proof.
-Admitted.
+  induction 2; inversion H; subst;
+    (* simplifying equality comes from binds *)
+    try match goal with
+    | E : _ = _ |- _ => inversion E
+    end; eauto with lc.
+Qed.
 
 (* 'inst' is short for 'instantiate' *)
 Reserved Notation "T ⊩ e1 ⇝ e2" (at level 65, e1 at level 58, no associativity).
@@ -172,9 +191,11 @@ Inductive inst_expr : subst_set → aexpr → bexpr → Prop :=
 | inste_var : forall Θ x,     wf_ss Θ → inst_expr Θ `′x `'x
 | inste_ex  : forall Θ x A e, wf_ss Θ → x : A ≔ e ∈ Θ → inst_expr Θ  `^x  e
 | inste_k   : forall Θ x k,   wf_ss Θ → x ≔ ⧼k⧽ ∈ Θ → inst_expr Θ ⧼`^x⧽ ⧼k⧽'
+| inste_star: forall Θ, wf_ss Θ → inst_expr Θ ⋆′ ⋆'
+| inste_box : forall Θ, wf_ss Θ → inst_expr Θ ◻′ ◻'
 | inste_num : forall Θ n,     wf_ss Θ → inst_expr Θ (ae_num n) (be_num n)
-| inste_int : forall Θ,       wf_ss Θ → inst_expr Θ ae_int be_int
-| inste_bot : forall Θ, inst_expr Θ ae_bot be_bot
+| inste_int : forall Θ, wf_ss Θ → inst_expr Θ ae_int be_int
+| inste_bot : forall Θ, wf_ss Θ → inst_expr Θ ae_bot be_bot
 | inste_app : forall Θ f' f a' a
   , inst_expr Θ f' f → inst_expr Θ a' a
   → inst_expr Θ (ae_app f' a') (be_app f a)
@@ -205,8 +226,11 @@ where "T ⊩ e1 ⇝ e2" := (inst_expr T e1 e2) : type_scope
 Lemma inst_e_wf_ss : forall Θ e' e,
     Θ ⊩ e' ⇝ e → wf_ss Θ.
 Proof.
-  admit.
-Admitted.
+  induction 1; pick fresh x'; eauto.
+Qed.
+
+#[export]
+Hint Resolve inst_e_wf_ss : core.
 
 Require Import Program.Tactics.
 
@@ -227,11 +251,10 @@ Lemma inst_e_lc : forall Θ e' e,
     Θ ⊩ e' ⇝ e → lc_bexpr e.
 Proof.
   induction 1; try solve [auto | pick fresh x; eauto 6 with lc].
-Admitted.
-
-
-#[export]
-Hint Resolve inst_e_wf_ss : core.
+  - apply wf_lc_sse in H0.
+    + now inversion H0.
+    + assumption.
+Qed.
 
 Reserved Notation "T ⊩ ob ⇝? dob" (at level 65, ob at level 58, no associativity).
 Inductive inst_obind : subst_set → obind → obindd → Prop :=
@@ -240,43 +263,43 @@ Inductive inst_obind : subst_set → obind → obindd → Prop :=
 where "T ⊩ ob ⇝? dob" := (inst_obind T ob dob) : type_scope
 .
 
-Reserved Notation "T ⊩ w1 ⇝′ w2" (at level 65, w1 at level 58).
+Reserved Notation "T1 ⊩ w1 ⇝′ w2 ⫣ T2" (at level 65, w1 at level 58).
 Reserved Notation "T1 ⊩ G1 ⟿ G2 ⫣ T2" (at level 65, G1 at level 58, G2 at level 58).
-Inductive inst_work : subst_set → work → dwork → Prop :=
+Inductive inst_work : subst_set → work → dwork → subst_set → Prop :=
 | instw_check : forall Θ ob ob' e1 e1' e2 e2' A A'
   , inst_obind Θ ob' ob → inst_expr Θ A' A
   → inst_expr Θ e1' e1 → inst_expr Θ e2' e2
-  → inst_work Θ (ob' ⊢? e1' <: e2' ⇐′ A') (ob ⊢? e1 <: e2 ⇐ A)
+  → inst_work Θ (ob' ⊢? e1' <: e2' ⇐′ A') (ob ⊢? e1 <: e2 ⇐ A) Θ
 | instw_cpct  : forall Θ A A' B B'
   , inst_expr Θ A' A → inst_expr Θ B' B
-  → inst_work Θ (A' ≲′ B') (A ≲ B)
+  → inst_work Θ (A' ≲′ B') (A ≲ B) Θ
 | instw_infer : forall L Θ Θ' e1 e1' e2 e2' c c'
   , inst_expr Θ e1' e1 → inst_expr Θ e2' e2
   → (forall x, x `notin` L → inst_wl Θ (c' $′ `′x) (c $ `'x) Θ')
-  → inst_work Θ (e1' <: e2' ⇒′ c') (e1 <: e2 ⇒ c)
+  → inst_work Θ (e1' <: e2' ⇒′ c') (e1 <: e2 ⇒ c) Θ'
 | instw_iapp : forall L Θ Θ' A A' e e1' e2' c c'
   , inst_expr Θ e1' e → inst_expr Θ e2' e
   → (forall x, x `notin` L → inst_wl Θ (c' $′ `′x) (c $ `'x) Θ')
-  → inst_work Θ (A' ⋅ e1' & e2' ⇒′ c') (A ⋅ e ⇒ c)
+  → inst_work Θ (A' ⋅ e1' & e2' ⇒′ c') (A ⋅ e ⇒ c) Θ'
 | instw_red : forall L Θ Θ' A A' c c'
   , inst_expr Θ A' A
   → (forall x, x `notin` L → inst_wl Θ (c' $′ `′x) (c $ `'x) Θ')
-  → inst_work Θ (A' ⟼′ c') (A ⟼ c)
-where "T ⊩ w1 ⇝′ w2" := (inst_work T w1 w2) : type_scope
+  → inst_work Θ (A' ⟼′ c') (A ⟼ c) Θ'
+where "T1 ⊩ w1 ⇝′ w2 ⫣ T2" := (inst_work T1 w1 w2 T2) : type_scope
 with inst_wl  : subst_set → worklist → dworklist → subst_set → Prop :=
 | instwl_nil  : forall Θ, inst_wl Θ wl_nil dwl_nil Θ
-| instwl_cons : forall Θ Θ' Γ Γ' w w'
-  , inst_wl Θ Γ' Γ Θ' → inst_work Θ' w' w
-  → inst_wl Θ (Γ' ⊨′ w') (Γ ⊨ w) Θ'
+| instwl_cons : forall Θ Θ' Θ'' Γ Γ' w w'
+  , inst_wl Θ Γ' Γ Θ' → inst_work Θ' w' w Θ''
+  → inst_wl Θ (Γ' ⊨′ w') (Γ ⊨ w) Θ''
 | instwl_var  : forall Θ Θ' Γ Γ' x A A'
-  , inst_wl Θ Γ' Γ Θ' → x `notin` dom Θ → inst_expr Θ' A' A
+  , inst_wl Θ Γ' Γ Θ' → x `notin` dom Θ' → inst_expr Θ' A' A
   → inst_wl Θ (Γ' ,′ x :′ A') (Γ ,′' x : A) (Θ'; x : A!)
 | instwl_kv : forall Θ Θ' Γ Γ' x k
-  , inst_wl Θ Γ' Γ Θ' → x `notin` dom Θ
+  , inst_wl Θ Γ' Γ Θ' → x `notin` dom Θ'
   → inst_wl Θ (Γ' ,′ ⧼^x⧽) Γ (Θ'; x ≔ ⧼k⧽)
 | instwl_ex : forall Θ Θ' Γ Γ' x A' A e
   , mono_btype e
-  → inst_wl Θ Γ' Γ Θ' → x `notin` dom Θ → inst_expr Θ' A' A
+  → inst_wl Θ Γ' Γ Θ' → x `notin` dom Θ' → inst_expr Θ' A' A
   → inst_wl Θ (Γ' ,′ ^x :′ A') Γ (Θ'; x : A ≔ e)
 where "T1 ⊩ G1 ⟿ G2 ⫣ T2" := (inst_wl T1 G1 G2 T2) : type_scope
 .
@@ -290,12 +313,33 @@ Definition transfer' (Γ' : worklist) (Γ : dworklist) : Prop :=
 
 Hint Extern 2 (_ = _) => simpl; congruence : core.
 
-Lemma inst_e_det : forall e' Θ e1 e2,
-  uniq Θ → Θ ⊩ e' ⇝ e1 → Θ ⊩ e' ⇝ e2 → e1 = e2.
+Lemma inst_e_det : forall e' Θ e1,
+  uniq Θ → Θ ⊩ e' ⇝ e1 → forall e2, Θ ⊩ e' ⇝ e2 → e1 = e2.
 Proof.
-Admitted.
+  intros * Uniq H1.
+  induction H1; intros e2 H2; inversion H2; subst; auto;
+  (* solving all the binds with binds_unique in metalib *)
+  try match goal with
+  | H1 : binds ?x ?e1 ?c , H2 : binds ?x ?e2 ?c |- _ = _ =>
+    let E := fresh "E" in
+      assert (e1 = e2) as E by (eapply binds_unique; eauto);
+      inversion E; now subst
+  end;
 
-
+  repeat match goal with
+  (* basic inductive cases *)
+  | H1 : _ ⊩ ?e ⇝ ?e1 , H2 : _ ⊩ ?e ⇝ ?e2 |- _ =>
+      assert (e1 = e2) by auto; clear H1 H2
+  (* inductive cases with locally nameless mess *)
+  | H1 : forall x, x `notin` ?L1 → _ ⊩ _ ⇝ ?e1 ^`' x
+  , H2 : forall x, x `notin` ?L2 → _ ⊩ _ ⇝ ?e2 ^`' x
+    |- _ => pick fresh x for
+      (L1 `union` L2 `union` fv_bexpr e1 `union` fv_bexpr e2);
+         assert (e1 ^`' x = e2 ^`' x) by eauto;
+         assert (e1 = e2) by (eapply open_bexpr_wrt_bexpr_inj; eauto)
+  end;
+  congruence.
+Qed.
 
 Lemma inst_wl_split : forall Γ1' Γ2' Γ Θ Θ'
   , Θ ⊩ Γ1' ⫢′ Γ2' ⟿ Γ ⫣ Θ'
@@ -305,51 +349,73 @@ Lemma inst_wl_split : forall Γ1' Γ2' Γ Θ Θ'
     ∧ Θ0 ⊩ Γ2' ⟿ Γ2 ⫣ Θ'.
 Proof.
   induction Γ2'; simpl; intros.
-  - exists Γ, dwl_nil, Θ'; simpl; solve [auto].
+  - exists Γ, dwl_nil, Θ'; simpl; auto.
   - inversion H; subst.
     pose proof (IHΓ2' _ _ _ H3) as (Γ1 & Γ2 & Θ0 & E & Inst1 & Inst2).
-    exists Γ1, (Γ2 ⊨ w0), Θ0. auto.
-  - destruct b.
-    + inversion H; subst.
-      pose proof (IHΓ2' _ _ _ H4) as (Γ1 & Γ2 & Θ0 & E & Inst1 & Inst2).
-      exists Γ1, (Γ2 ,' x : A0), Θ0. admit.
-    + inversion H; subst.
-      pose proof (IHΓ2' _ _ _ H5) as (Γ1 & Γ2 & Θ0 & E & Inst1 & Inst2).
-      exists Γ1, Γ2, Θ0. admit.
-    + inversion H; subst.
-      pose proof (IHΓ2' _ _ _ H3) as (Γ1 & Γ2 & Θ0 & E & Inst1 & Inst2).
-      exists Γ1, Γ2, Θ0. admit.
-Admitted.
+    exists Γ1, (Γ2 ⊨ w0), Θ0. repeat split; eauto.
+  - destruct b; inversion H; subst.
+    + pose proof (IHΓ2' _ _ _ H4) as (Γ1 & Γ2 & Θ0 & E & Inst1 & Inst2).
+      exists Γ1, (Γ2 ,′' x : A0), Θ0.
+      subst. repeat split; auto.
+    + pose proof (IHΓ2' _ _ _ H5) as (Γ1 & Γ2 & Θ0 & E & Inst1 & Inst2).
+      exists Γ1, Γ2, Θ0.
+      subst. repeat split; auto.
+    + pose proof (IHΓ2' _ _ _ H3) as (Γ1 & Γ2 & Θ0 & E & Inst1 & Inst2).
+      exists Γ1, Γ2, Θ0.
+      subst. repeat split; auto.
+Qed.
 
 Scheme wl_mut   := Induction for worklist Sort Prop
   with work_mut := Induction for work     Sort Prop.
 
-Scheme wins_mut   := Induction for inst_work Sort Prop
+Scheme winst_mut   := Induction for inst_work Sort Prop
   with wlinst_mut := Induction for inst_wl   Sort Prop.
 
-Lemma inst_wl_ss_expand : forall Θ Γ' Γ Θ'
+Lemma inst_wl_ss_extend : forall Θ Γ' Γ Θ'
   , Θ ⊩ Γ' ⟿ Γ ⫣ Θ'
   → exists Θ0, Θ ;; Θ0 = Θ'.
 Proof.
-  induction 1; try pose proof IHinst_wl as (Θ0 & <-).
+  intros * H.
+  pattern Θ, Γ', Γ, Θ', H.
+  apply wlinst_mut with
+    (P := fun Θ w' w Θ' (_ : Θ ⊩ w' ⇝′ w ⫣ Θ') => exists Θ0, Θ ;; Θ0 = Θ');
+    intros.
+
   - now exists nil.
-  - assumption.
-  - now exists (Θ0; x : A !).
-  - now exists (Θ0; x ≔ ⧼k⧽).
-  - now exists (Θ0; x : A ≔ e).
+  - now exists nil.
+  - pick fresh x. eauto.
+  - pick fresh x. eauto.
+  - pick fresh x. eauto.
+  - now exists nil.
+
+  - destruct H0. destruct H1. subst. now exists (x ;; x0).
+  - destruct H0. subst. now exists (x0; x : A !).
+  - destruct H0. subst. now exists (x0; x ≔ ⧼k⧽).
+  - destruct H0. subst. now exists (x0; x : A ≔ e).
 Qed.
 
-Lemma inst_e_weakening : forall Θ e' e Θ',
-  Θ ⊩ e' ⇝ e → Θ ;; Θ' ⊩ e' ⇝ e.
+Lemma inst_w_ss_extend : forall Θ w' w Θ'
+  , Θ ⊩ w' ⇝′ w ⫣ Θ'
+  → exists Θ0, Θ ;; Θ0 = Θ'.
 Proof.
-  induction 1; eauto.
-Admitted.
+  induction 1; solve
+    [now exists nil
+    | pick fresh x; eauto using inst_wl_ss_extend].
+Qed.
+
+Lemma inst_e_weakening : forall Θ1 Θ2 e' e Θ'
+  , Θ1 ;; Θ2 ⊩ e' ⇝ e → wf_ss (Θ1 ;; Θ' ;; Θ2)
+  → Θ1 ;; Θ' ;; Θ2 ⊩ e' ⇝ e.
+Proof.
+  intros * H.
+  dependent induction H; intros; eauto 4.
+Qed.
 
 #[local]
 Hint Resolve inst_e_weakening : inst_weakening.
 
-Lemma inst_ob_weakening : forall Θ Θ' ob' ob,
-  Θ ⊩ ob' ⇝? ob → Θ ;; Θ' ⊩ ob' ⇝? ob.
+Lemma inst_ob_weakening : forall Θ1 Θ2 Θ' ob' ob,
+  Θ1 ;; Θ2 ⊩ ob' ⇝? ob → Θ1 ;; Θ' ;; Θ2 ⊩ ob' ⇝? ob.
 Proof.
   induction 1; eauto.
 Qed.
@@ -357,36 +423,179 @@ Qed.
 #[local]
 Hint Resolve inst_ob_weakening : inst_weakening.
 
-(* doable *)
-Lemma inst_w_weakening : forall Θ w' w Θ',
-  Θ ⊩ w' ⇝′ w → Θ ;; Θ' ⊩ w' ⇝′ w.
+Lemma wf_ss_unapp : forall xs ys,
+    wf_ss (xs ;; ys) → wf_ss xs.
 Proof.
-  intros.
-  pattern Θ, w', w, H.
-  apply wins_mut with
-      (P0 := fun Θ Γ' Γ Θ1 (_ : Θ ⊩ Γ' ⟿ Γ ⫣ Θ1) =>
-               forall Θ0, Θ1 = Θ ;; Θ0 → Θ ⊩ Γ' ⟿ Γ ⫣ Θ ;; Θ0 → Θ ;; Θ' ⊩ Γ' ⟿ Γ ⫣ Θ ;; Θ' ;; Θ0);
-    intros.
-Admitted.
+  induction ys; intros.
+  - assumption.
+  - inversion H; auto.
+Qed.
 
-Lemma inst_e_rev_subst : forall v' v x e' e0 Θ
-  , Θ ⊩ [v' /′ x] e' ⇝ e0 → Θ ⊩ v' ⇝ v
-  → exists e, [v /' x] e = e0 ∧ Θ ⊩ e' ⇝ e.
+Lemma wf_ss_uncons : forall xs x,
+    wf_ss (x :: xs) → wf_ss xs.
+Proof.
+  destruct x; inversion 1; auto.
+Qed.
+
+
+Hint Immediate wf_ss_unapp wf_ss_uncons : inst_weakening.
+
+Ltac clear_app_suffix_impl :=
+  match goal with
+  | H : ?xs = ?ys ++ ?xs |- _ =>
+      assert (ys = nil) as -> by
+        now apply app_nil_invert in H
+  | H : ?ys ++ ?xs = ?xs |- _ =>
+      symmetry in H
+  | H : ?ys ++ ?xs = ?zs ++ ?xs |- _ =>
+      apply app_inj_l in H
+  | H : ?ys1 ++ ?ys2 ++ ?xs = ?zs ++ ?xs |- _ =>
+      rewrite (app_assoc ys1 ys2 xs) in H
+  | H : ?zs ++ ?xs = ?ys1 ++ ?ys2 ++ ?xs |- _ =>
+      symmetry in H
+  | H : ?x :: ?ys ++ ?xs = ?zs ++ ?xs |- _ =>
+      rewrite <- (cons_app_assoc _ x ys xs) in H;
+      clear_app_suffix_impl
+  end; simpl in *
+.
+
+Ltac clear_app_suffix :=
+  repeat progress clear_app_suffix_impl.
+
+Ltac simplify_list_eq :=
+  repeat (subst || clear_app_suffix);
+  repeat rewrite <- app_assoc in *;
+  simpl in *.
+
+Ltac conclude_ss_extend_impl :=
+  let process t1 t2 tac :=
+    let t3 := fresh "Θ" in
+    let E  := fresh "E" in
+    lazymatch t2 with
+    (* t2 is already an extension of t1 *)
+    | t1 ;; ?t => fail
+    | _ =>
+        lazymatch goal with
+        (* the equality we want to conclude already exists *)
+        | _ : t1 ;; ?t = t2 |- _ => fail
+        (* doing actual stuff *)
+        | _ => assert (exists t, t1 ;; t = t2) as [t3 E] by tac
+        end
+    end
+  in
+  match goal with
+  | H : ?t1 ⊩ _ ⟿ _ ⫣ ?t2 |- _ =>
+      process t1 t2 ltac:(eapply inst_wl_ss_extend; eassumption)
+  | H : ?t1 ⊩ _ ⇝′ _ ⫣ ?t2 |- _ =>
+      process t1 t2 ltac:(eapply inst_w_ss_extend; eassumption)
+  end
+.
+
+Ltac conclude_ss_extend :=
+  repeat conclude_ss_extend_impl.
+
+Lemma inst_wl_weakening : forall Θ1 Θ2 Θ3 Γ' Γ
+  , Θ1 ;; Θ2 ⊩ Γ' ⟿ Γ ⫣ Θ1 ;; Θ2 ;; Θ3
+  → forall Θ', wf_ss (Θ1 ;; Θ' ;; Θ2 ;; Θ3)
+  → Θ1 ;; Θ' ;; Θ2 ⊩ Γ' ⟿ Γ ⫣ Θ1 ;; Θ' ;; Θ2 ;; Θ3.
 Proof.
   intros * H.
-  assert (lc_aexpr e') by admit.
-  generalize dependent e0. generalize dependent Θ.
-  induction H0; simpl; intros.
-  - exists (` x0). simpl. destruct (x0 == x).
-    + admit.
-    + admit.
-  - admit.
-  - admit.
-  - admit.
-  - admit.
-  - admit.
-  - admit.
-  - admit.
+  (* manual dependent mutual induction *)
+  remember (Θ1 ;; Θ2 ;; Θ3) as Θ'.
+  remember (Θ1 ;; Θ2) as Θ.
+  generalize dependent Θ3;
+  generalize dependent Θ2;
+  generalize dependent Θ1.
+  pattern Θ, Γ', Γ, Θ', H.
+  apply wlinst_mut with
+    (P := fun Θ w' w Θ0 (_ : Θ ⊩ w' ⇝′ w ⫣ Θ0) =>
+      forall Θ1 Θ2 Θ3 Θ', Θ = Θ1 ;; Θ2 → Θ0 = Θ1 ;; Θ2 ;; Θ3
+      → wf_ss (Θ1 ;; Θ' ;; Θ2 ;; Θ3)
+      → Θ1 ;; Θ' ;; Θ2 ⊩ w' ⇝′ w ⫣ Θ1 ;; Θ' ;; Θ2 ;; Θ3);
+    intros; subst.
+
+  (* inst_w *)
+  - clear_app_suffix; eauto 6 with inst_weakening.
+  - clear_app_suffix; eauto 6 with inst_weakening.
+  - eauto with inst_weakening.
+  - eauto with inst_weakening.
+  - eauto with inst_weakening.
+
+  (* inst_wl *)
+  - clear_app_suffix. auto.
+  - conclude_ss_extend. simplify_list_eq.
+    eapply instwl_cons.
+    + eauto with inst_weakening.
+    + replace (Θ1;; Θ'1;; Θ2;; Θ0;; Θ4) with
+        (Θ1;; Θ'1;; (Θ2;; Θ0);; Θ4) by
+        now repeat rewrite <- app_assoc.
+    rewrite (app_assoc Θ0 Θ2 (Θ1 ;; Θ'1)).
+    apply H1; eauto 4; rewrite <- app_assoc; auto.
+  - conclude_ss_extend; simplify_list_eq.
+    inversion H1; subst; constructor; auto.
+    + rewrite app_assoc; apply inst_e_weakening;
+      now rewrite <- app_assoc.
+  - conclude_ss_extend; simplify_list_eq.
+    inversion H1; subst. constructor; auto.
+  - conclude_ss_extend; simplify_list_eq.
+    inversion H1; subst. constructor; auto.
+    + rewrite app_assoc; apply inst_e_weakening;
+       now rewrite <- app_assoc.
+Qed.
+
+Hint Resolve inst_wl_weakening : inst_weakening.
+
+Lemma inst_w_weakening : forall Θ1 Θ2 Θ3 w' w
+  , Θ1 ;; Θ2 ⊩ w' ⇝′ w ⫣ Θ1 ;; Θ2 ;; Θ3
+  → forall Θ', wf_ss (Θ1;; Θ';; Θ2 ;; Θ3)
+  → Θ1 ;; Θ' ;; Θ2 ⊩ w' ⇝′ w ⫣ Θ1 ;; Θ' ;; Θ2 ;; Θ3.
+Proof.
+  intros * H.
+  dependent induction H; intros;
+    clear_app_suffix; eauto 6 with inst_weakening.
+Qed.
+
+
+Lemma inst_e_rev_subst : forall v' v x e'
+  , lc_aexpr e' → forall e0 Θ, x `notin` fv_bexpr e0
+  → Θ ⊩ [v' /′ x] e' ⇝ e0 → Θ ⊩ v' ⇝ v
+  → exists e, [v /' x] e = e0 ∧ Θ ⊩ e' ⇝ e.
+Proof.
+  intros * Lc.
+  induction Lc; simpl; intros * Fr He Hv.
+  - exists (`' x0). simpl.
+    unfold eq_dec in *. destruct (EqDec_eq_of_X x0 x).
+    + assert (v = e0) by (eapply inst_e_det with (Θ := Θ); eauto).
+      eauto.
+    + inversion He. now subst.
+  - destruct k; inversion He; subst.
+    + exists ⋆'; eauto.
+    + exists ◻'; eauto.
+    + exists ⧼ k ⧽'; eauto.
+  - inversion He. subst.
+    exists e0. eauto with lngen.
+  - inversion He. subst.
+    exists (be_num n); eauto.
+  - inversion He. subst.
+    exists be_int; eauto.
+  - inversion He; subst.
+    exists be_bot; eauto.
+  - inversion He. subst. simpl in Fr.
+    edestruct (IHLc1 f) as (e1' & E1 & Trans1); eauto.
+    edestruct (IHLc2 a) as (e2' & E2 & Trans2); eauto.
+    exists (be_app e1' e2'). simpl. split. congruence.
+    eauto.
+  - inversion He. subst. simpl in Fr.
+    pick fresh x' for (add x L).
+    assert (Θ ⊩ ([v' /′ x] e) ^`′ x' ⇝ e1 ^`' x').
+    eapply H3. auto.
+    assert (([v' /′ x] e) ^`′ x' = [v' /′ x] e ^`′ x') by admit.
+    rewrite H2 in H1.
+    destruct (H0 x' (e1 ^`' x') Θ) as (e1' & E & Trans).
+    admit. auto. auto.
+    exists (be_abs (close_bexpr_wrt_bexpr x' e1')). split.
+    simpl. admit.
+    econstructor. intros. admit.
   - admit.
 Admitted.
 
@@ -412,4 +621,3 @@ Proof.
   - admit.
   -
 Admitted.
-*)
