src-lite/lc.v
@@ -1,0 +1,8 @@
+Require Import bidir_notations.
+
+Lemma mono_lc_bexpr : forall e, mono_btype e → lc_bexpr e.
+Proof.
+  induction 1; eauto.
+Qed.
+
+Hint Resolve mono_lc_bexpr : lc.
