src-lite/list_properties.v
@@ -1,0 +1,30 @@
+Require Export Lists.List.
+Require Import Utf8.
+
+Import ListNotations.
+
+Lemma app_r_cons : forall {A} {a : A} xs ys,
+    xs ++ a :: ys = (xs ++ [a]) ++ ys.
+Proof.
+  intros. now rewrite <- app_assoc.
+Qed.
+
+Lemma app_inj_l : forall A (xs ys zs : list A),
+    ys ++ xs = zs ++ xs → ys = zs.
+Proof.
+  induction xs; intros.
+  - now repeat rewrite app_nil_r in H.
+  - rewrite (app_r_cons ys xs) in H.
+    rewrite (app_r_cons zs xs) in H.
+    apply IHxs in H.
+    now apply app_inj_tail_iff in H as (? & ?).
+Qed.
+
+Lemma app_nil_invert : forall A (xs ys : list A),
+    xs = ys ++ xs -> ys = [].
+Proof.
+  intros.
+  replace xs with (nil ++ xs) in H at 1.
+  - now apply app_inj_l in H.
+  - auto.
+Qed.
